\begin{tabular}{|l|c l|c l|}
    \hline
    & (a) & & (b) & \\
    \hline
    Postulate 2 & $x + 0 = x$ & & $x \cdot 1 = x$ & \\
    \hline
    Postulate 5 & $x + x' = 1$ & & $x
    \cdot x' = 0$ & \\
    \hline
    Theorem 1 & $x + x = x$ & & $x \cdot x = x$ & \\
    \hline
    Theorem 2 & $x + 1 = 1$ & & $x \cdot 0 = 0$ & \\
    \hline
    Theorem 3, involution & $(x')' = x$ & & - & \\
    \hline
    Postulate 3, commutative & $x + y = y + x$ & & $xy = yx$ & \\
    \hline
    Theorem 4, associative & $x + (y + z) = (x + y) + z$ & & $x(yz) = (xy)z$ & \\
    \hline
    Postulate 4, distributive & $x(y + z) = xy + xz$ & & $x + yz = (x + y)(x + z)$ & \\
    \hline
    Theorem 5, DeMorgan & $(x + y)' = x' y'$ & & $(xy)' = x' + y'$ & \\
    \hline
    Theorem 6, absorption & $x + xy = x$ & & $x(x + y) = x$ & \\
    \hline
\end{tabular}
